fairness/lawyer/obls_utils.v
@@ -1,0 +1,76 @@
+From stdpp Require Import relations.
+From iris.proofmode Require Import tactics.
+
+(* TODO: find existing definition *)
+Definition rel_compose {A: Type} (R1 R2 : relation A): relation A :=
+  fun x y => exists z, R1 x z /\ R2 z y.
+
+(* TODO: find existing *)
+Global Instance rel_subseteq {A: Type}: SubsetEq (relation A) :=
+  fun R1 R2 => forall x y, R1 x y -> R2 x y. 
+
+Global Instance rel_compose_mono {A: Type}:
+  Proper (subseteq ==> subseteq ==> subseteq) (@rel_compose A).
+Proof.
+  red. intros ??????. rewrite /rel_compose.
+  red. intros ?? (?&?&?). eexists. eauto.
+Qed.
+
+Lemma nsteps_0 {A} (R: relation A) x y: nsteps R 0 x y <-> x = y.
+Proof.
+  split.
+  - intros STEP. by inversion STEP.
+  - intros ->. constructor.
+Qed. 
+
+Lemma nsteps_1 {A} (R: relation A) x y: nsteps R 1 x y <-> R x y.
+Proof.
+  split.
+  - intros STEP. inversion STEP; subst. inversion H1. by subst. 
+  - intros. econstructor; eauto. constructor. 
+Qed. 
+
+Lemma rel_compose_nsteps_next' {A: Type} (r: relation A) n:
+  forall x y,
+    rel_compose r (relations.nsteps r n) x y <->
+      relations.nsteps r (S n) x y.
+Proof using.
+  intros. split.
+  - intros (?&?&?). econstructor; eauto.
+  - intros STEP. inversion STEP. subst. eexists. eauto.
+Qed. 
+
+Lemma rel_compose_assoc {A: Type} (R1 R2 R3: relation A):
+  forall x y,
+    rel_compose (rel_compose R1 R2) R3 x y <-> rel_compose R1 (rel_compose R2 R3) x y.
+Proof.
+  intros. rewrite /rel_compose. set_solver.
+Qed. 
+
+Lemma rel_compose_nsteps_plus {A: Type} (r: relation A) n m:
+  forall x y,
+    rel_compose (relations.nsteps r n) (relations.nsteps r m) x y <->
+      relations.nsteps r (n + m) x y.
+Proof using.
+  intros. generalize dependent y. generalize dependent x. induction n; intros.
+  { rewrite /rel_compose. simpl. setoid_rewrite nsteps_0. set_solver. }    
+  rewrite Nat.add_succ_l -rel_compose_nsteps_next'. 
+  rewrite /rel_compose. setoid_rewrite <- rel_compose_nsteps_next'.
+  setoid_rewrite rel_compose_assoc. rewrite /rel_compose.
+  by setoid_rewrite IHn. 
+Qed. 
+
+Lemma rel_compose_nsteps_next {A: Type} (r: relation A) n:
+  forall x y,
+    rel_compose (relations.nsteps r n) r x y <->
+      relations.nsteps r (S n) x y.
+Proof using.
+  intros. rewrite /rel_compose.
+  setoid_rewrite <- (nsteps_1 r). setoid_rewrite rel_compose_nsteps_plus.
+  f_equiv. lia. 
+Qed. 
+
+Global Instance rel_subseteq_po {A: Type}: PreOrder (@rel_subseteq A).
+Proof.
+  rewrite /rel_subseteq. split; eauto.
+Qed.
